src/Path.v
@@ -9,17 +9,37 @@ Import Wf_nat.
 
 Import Utils.
 
+(** * Path Module *)
+
+(** This module defines and manipulates paths, represented as lists of natural numbers.
+    It provides basic structural operations (like splitting and equality),
+    as well as a custom induction principle based on list suffix decomposition. *)
 Module Path.
+  (** ** Definition of Paths *)
+  (** A [path] is represented as a list of natural numbers. *)
   Definition path := list nat.
 
+  (** ** Path Splitting *)
+    
+  (** [path_sep] decomposes a non-empty list into its prefix (all elements except the last)
+      and its final element. It returns [None] if the list is empty. *)
+  Definition path_sep {T: Type} (l: list T) :=
+    match l with
+    | [] => None
+    | hd :: _ => Some (removelast l, last l hd)
+    end.
 
-  Lemma list_sep_None : forall T (l: list T), list_sep l = None <-> l = [].
+  (** ** Properties of [path_sep] *)
+
+  (** [path_sep_None]: [path_sep l] yields [None] if and only if [l] is empty. *)
+  Lemma path_sep_None : forall T (l: list T), path_sep l = None <-> l = [].
   Proof.
     split; intros.
     - destruct l; [reflexivity | discriminate H].
     - subst. reflexivity.
   Qed.
 
+  (** [removelast_length]: Removing the last element of a non-empty list strictly reduces its length. *)
   Lemma removelast_length : forall T (l: list T), l <> [] -> length (removelast l) < length l.
   Proof.
     induction l; intros.
@@ -30,32 +50,43 @@ Module Path.
         rewrite Hl. unfold not. intros. discriminate H0.
   Qed.
 
-  Lemma list_sep_Some : forall T (l: list T) x l',
-      list_sep l = Some (l', x) <-> l = l' ++ [x] /\ length l' < length l.
+  (** [path_sep_Some]: When [path_sep l] = [Some (l', x)], the list [l] equals [l' ++ [x]],
+    and the length of [l'] is strictly less than that of [l]. *)
+  Lemma path_sep_Some : forall T (l: list T) x l',
+      path_sep l = Some (l', x) <-> l = l' ++ [x] /\ length l' < length l.
   Proof.
     split; intros.
     - destruct l eqn:Hl.
       + discriminate H.
-      + unfold list_sep in H. rewrite <- Hl in *. inversion H. split.
+      + unfold path_sep in H. rewrite <- Hl in *. inversion H. split.
         * apply app_removelast_last. unfold not. intros. subst. discriminate H0.
         * apply removelast_length. subst. discriminate.
     - destruct l eqn:Hl; destruct H.
       + apply app_cons_not_nil in H. contradiction.
-      + unfold list_sep. rewrite <- Hl in *. assert (HlNil: l <> []). subst. discriminate.
+      + unfold path_sep. rewrite <- Hl in *. assert (HlNil: l <> []). subst. discriminate.
         apply app_removelast_last with (d := t) in HlNil. rewrite HlNil in H.
         rewrite app_inj_tail_iff in H. destruct H. subst. reflexivity.
   Qed.
 
+  (** ** Induction Principle on Paths *)
+  
+  (**
+    [path_ind] defines a structural induction principle for paths that proceeds
+    by successively removing the last element of the list.
+    It enables reasoning over paths constructed by appending elements at the end,
+    rather than at the front. *)
   Theorem path_ind : forall (P : path -> Prop), P [] -> (forall x l, P l -> P (l ++ [x])) -> forall p, P p.
   Proof.
     intros. induction p using (induction_ltof1 _ (@length _)). unfold ltof in H1.
-    destruct (list_sep x) as [[a b]|] eqn:Hp.
-    - apply list_sep_Some in Hp. destruct Hp as [Hp Hlen].
+    destruct (path_sep x) as [[a b]|] eqn:Hp.
+    - apply path_sep_Some in Hp. destruct Hp as [Hp Hlen].
       rewrite Hp. apply H0. apply H1. assumption.
-    - apply list_sep_None in Hp. subst. assumption.
+    - apply path_sep_None in Hp. subst. assumption.
   Qed.
 
+  (** ** Decidability *)
+  
+  (** [path_eq_dec]: Equality over paths (lists of naturals) is decidable. *)
   Theorem path_eq_dec : forall (a b: path), {a = b} + {a <> b}.
-  Proof. decide equality. decide equality.  Qed.
-
+  Proof. decide equality. decide equality. Qed.
 End Path.
