src/Extr.v
@@ -7,10 +7,4 @@ Import Algo.
 Extraction Language OCaml.
 Set Extraction Output Directory ".".
 
-Extract Inductive list => "list" [ "[]" "(::)" ].
-Extract Inductive nat => "int" [ "0" "succ" ].
-
-Extract Constant Nat.add => "( + )".
-Extract Constant Nat.mul => "( * )".
-Extract Constant Nat.max => "(fun x y -> max x y)".
-
+Recursive Extraction type.
