src/Utils.v
@@ -7,11 +7,15 @@ From Stdlib Require Import Classes.RelationClasses.
 Import Nat.
 Import ListNotations.
 
+(** Module imported from coq-tricks.
+    Provides a mechanism to store learnt hypotheses to avoid re-deriving
+    the same facts repeatedly during proof automation. *)
 Module Learn.
-  (* Taken from coq-tricks *)
+  (** A wrapper type used to record that a proposition [P] has been learnt. *)
   Inductive Learnt {P:Prop} :=
   | AlreadyLearnt (H:P).
 
+  (** Internal tactic: marks a hypothesis as learnt if it hasn’t been recorded yet. *)
   Local Ltac learn_fact H :=
     let P := type of H in
     lazymatch goal with
@@ -20,42 +24,126 @@ Module Learn.
     | _ => pose proof H; pose proof (AlreadyLearnt H)
     end.
 
+  (** Public interface for [learn_fact]. 
+      Usage: [learn H] records the fact [H] as already known. *)
   Tactic Notation "learn" constr(H) := learn_fact H.
 End Learn.
 
+(** Utility module providing:
+    - Custom Ltac tactics for common proof patterns.
+    - Helper lemmas for reasoning about lists and natural numbers.
+    - Definitions of indexed mapping functions and option-based ordering. *)
 Module Utils.
   Import Learn.
 
+  (** ** Custom tactics *)
+
+  (** [inv H]: performs inversion on hypothesis [H], clears it, and substitutes
+      resulting equalities into the context. *)
   Ltac inv H := inversion H; clear H; subst.
 
+  (** [antisym]: applies antisymmetry on a pair of [<=] relations in the context
+      and records the resulting equality using [learn]. *)
   Ltac antisym :=
     match goal with
     | [ H: ?x <= ?y, F: ?y <= ?x |- _ ] =>
         learn (le_antisymm _ _ H F)
-    end
-  .
+    end.
 
+  (** [splitHyp]: destructs a conjunction in the context. *)
   Ltac splitHyp :=
     match goal with
     | [ H: _ /\ _ |- _ ] => destruct H
-    end
-  .
-
+    end.
+  
+  (** [existsHyp]: destructs an existential hypothesis in the context. *)
   Ltac existsHyp :=
     match goal with
     | [ H: ex _ |- _ ] => destruct H
-    end
-  .
+    end.
 
+  (** Lemma and tactic to help build conjunctions incrementally. *)
+  Lemma and_with_impl : forall P Q, P -> (P -> Q) -> P /\ Q.
+  Proof.
+    split; intros; auto.
+  Qed.
+
+  (** [splitAnd]: prepares the goal for proving a conjunction by introducing
+      the left-hand side immediately and the right-hand side later. *)
+  Ltac splitAnd :=
+    match goal with
+    | [ |- _ /\ _ ] => apply and_with_impl; [idtac|intros]
+    end.
+
+  (** ** Reasoning on [max] *)
+
+  (** Decomposes the [max] function into explicit cases, preserving order relations. *)
+  Lemma max_dec_bis: forall a b, (max a b = a /\ b <= a) \/ (max a b = b /\ a <= b).
+  Proof.
+    intros.
+    destruct (max_dec a b).
+    - rewrite e. left. split. reflexivity. apply max_l_iff. assumption.
+    - rewrite e. right. split. reflexivity. apply max_r_iff. assumption.
+  Qed.
+
+  (** Auxiliary tactic used by [splitMax] to destruct results of [max_dec_bis]. *)
+  Ltac _useMaxDecBis :=
+    match goal with
+    | [ H: (_ = _ /\ _) \/ (_ = _ /\ _) |- _ ] =>
+        destruct H as [[?Heq ?H]|[?Heq ?H]]; rewrite Heq in *; clear Heq
+    end.
+
+  (** [splitMax]: applies [max_dec_bis] to all occurrences of [max x y] in either
+      the goal or context, and simplifies the resulting branches. *)
+  Ltac splitMax :=
+    match goal with
+    | [ H: context[max ?x ?y] |- _ ] => learn (max_dec_bis x y); _useMaxDecBis
+    | [ |- context[max ?x ?y] ] => learn (max_dec_bis x y); _useMaxDecBis
+    end.
+
+  (** ** List reasoning *)
+
+  (** Lemma stating that if two lists have the same length, then for every element
+      in one list accessible via [nth_error], there exists a corresponding element
+      at the same index in the other list. *)
+  Lemma nth_error_lists : forall A B (l: list A) (l': list B) n x,
+      nth_error l n = Some x -> length l = length l' -> exists y, nth_error l' n = Some y.
+  Proof.
+    induction l; intros.
+    - destruct n; discriminate H.
+    - destruct l'. discriminate H0. inv H0. destruct n.
+      + eexists. reflexivity.
+      + firstorder.
+  Qed.
+
+  (** [gen_nth]: given two lists of equal length and an index known to exist in one,
+      generates the corresponding element in the other list. *)
+  Ltac gen_nth :=
+    match goal with
+    | [ Hlen: length ?l1 = length ?l2, Hnth: nth_error ?l1 ?n = Some _ |- _ ] =>
+        destruct (nth_error_lists _ _ _ _ _ _ Hnth Hlen); clear Hlen
+    | [ Hlen: length ?l2 = length ?l1, Hnth: nth_error ?l1 ?n = Some _ |- _ ] =>
+        let HnewTh := fresh in assert(HnewTh: exists y, nth_error l2 n = Some y) by
+          (apply (nth_error_lists _ _ _ _ _ _ Hnth); symmetry; apply Hlen);
+                               destruct HnewTh; clear Hlen
+    end.
+  
+  (** ** Indexed mapping function *)
+
+  (** [mapI'] applies a function [f] to each element of a list [l],
+      passing its index (starting from [i]) as an additional argument. *)
   Fixpoint mapI'{X Y: Type} f i (l: list X) : list Y :=
     match l with
     | [] => []
     | hd :: tl => f i hd :: mapI' f (i + 1) tl
-    end
-  .
+    end.
 
+  (** [mapI] is a specialization of [mapI'] starting from index 0. *)
   Definition mapI {X Y: Type} (f: nat -> X -> Y) := mapI' f 0.
 
+  (** Characterization of elements in [mapI']: 
+      an element [y] appears in [mapI' f i l] iff there exists an index [n]
+      and element [x] such that [nth_error l n = Some x] and [y = f (i + n) x]. *)
   Lemma mapI'_values : forall (X Y: Type) (f: nat -> X -> Y) (l: list X) y i,
       In y (mapI' f i l) <-> exists n x, nth_error l n = Some x /\ y = f (i + n) x.
   Proof.
@@ -74,44 +162,24 @@ Module Utils.
           rewrite HNat. apply H2.
   Qed.
 
+  (** Simplified version of [mapI'_values] for the common case where indexing starts at 0. *)
   Lemma mapI_values :  forall (X Y: Type) (f: nat -> X -> Y) (l: list X) y,
       In y (mapI f l) <-> exists n x, nth_error l n = Some x /\ y = f n x.
   Proof.
     intros. unfold mapI. apply mapI'_values.
   Qed.
+  
+  (** ** Custom helper functions *)
 
-  Fixpoint maxList x l :=
-    match l with
-    | [] => x
-    | hd :: tl => max hd (maxList x tl)
-    end
-  .
-
+  (** Computes the sum of a list of natural numbers. *)
   Fixpoint sum (l: list nat) :=
     match l with
     | [] => 0
     | hd :: tl => hd + sum tl
-    end
-  .
+    end.
 
-  Lemma and_with_impl : forall P Q, P -> (P -> Q) -> P /\ Q.
-  Proof.
-    split; intros; auto.
-  Qed.
-
-  Ltac splitAnd :=
-    match goal with
-    | [ |- _ /\ _ ] => apply and_with_impl; [idtac|intros]
-    end
-  .
-
-  Definition list_sep {T: Type} (l: list T) :=
-    match l with
-    | [] => None
-    | hd :: _ => Some (removelast l, last l hd)
-    end
-  .
-
+  (** Defines an ordering relation on optional natural numbers,
+      treating [None] as the smallest element. *)
   Definition le_option_nat (x y : option nat) : Prop :=
     match x, y with
     | None, _ => True
@@ -119,58 +187,9 @@ Module Utils.
     | Some a, Some b => a <= b
     end.
 
+  (** [le_option_nat] is reflexive. *)
   Instance le_option_nat_Reflexive : Reflexive le_option_nat.
   Proof.
     intros [n|]; simpl; auto.
-  Qed.
-
-  Lemma max_dec_bis: forall a b, (max a b = a /\ b <= a) \/ (max a b = b /\ a <= b).
-  Proof.
-    intros.
-    destruct (max_dec a b).
-    - rewrite e. left. split. reflexivity. apply max_l_iff. assumption.
-    - rewrite e. right. split. reflexivity. apply max_r_iff. assumption.
-  Qed.
-
-  Ltac _useMaxDecBis :=
-    match goal with
-    | [ H: (_ = _ /\ _) \/ (_ = _ /\ _) |- _ ] =>
-        destruct H as [[?Heq ?H]|[?Heq ?H]]; rewrite Heq in *; clear Heq
-    end
-  .
-
-  Ltac splitMax :=
-    match goal with
-    | [ H: context[max ?x ?y] |- _ ] => learn (max_dec_bis x y); _useMaxDecBis
-    | [ |- context[max ?x ?y] ] => learn (max_dec_bis x y); _useMaxDecBis
-    end
-  .
-
-  Lemma nth_error_lists : forall A B (l: list A) (l': list B) n x,
-      nth_error l n = Some x -> length l = length l' -> exists y, nth_error l' n = Some y.
-  Proof.
-    induction l; intros.
-    - destruct n; discriminate H.
-    - destruct l'. discriminate H0. inv H0. destruct n.
-      + eexists. reflexivity.
-      + firstorder.
-  Qed.
-
-  Ltac gen_nth :=
-    match goal with
-    | [ Hlen: length ?l1 = length ?l2, Hnth: nth_error ?l1 ?n = Some _ |- _ ] =>
-        destruct (nth_error_lists _ _ _ _ _ _ Hnth Hlen); clear Hlen
-    | [ Hlen: length ?l2 = length ?l1, Hnth: nth_error ?l1 ?n = Some _ |- _ ] =>
-        let HnewTh := fresh in assert(HnewTh: exists y, nth_error l2 n = Some y) by
-          (apply (nth_error_lists _ _ _ _ _ _ Hnth); symmetry; apply Hlen);
-                               destruct HnewTh; clear Hlen
-    end
-  .
-
-  Lemma option_eq_dec : forall (T: Type) (x y: option T),
-      (forall x y: T, {x = y} + {x <> y}) -> {x = y} + {x <> y}.
-  Proof.
-    intros. destruct x; destruct y; try (destruct (X t0 t1)); subst;
-      left + right; congruence.
   Qed.
 End Utils.
